Iterator/Producers.lean
@@ -5,7 +5,6 @@ Authors: Paul Reichert
 -/
 prelude
 import Iterator.Basic
-import Iterator.Wrapper
 import Init.Data.Nat.Lemmas
 
 section ListIterator
@@ -41,17 +40,6 @@ structure ListIterator (α : Type u) where
 --     cases it
 --     split at h <;> simp_all [IterStep.successor]
 
-instance {α : Type u} [Pure m] [UnivLE.{u, w}] : Iterator (ListIterator α) m α where
-  state_small := inferInstance
-  value_small := inferInstance
-  plausible_step it
-    | .yield it' out => it.list = out :: it'.list
-    | .skip _ => False
-    | .done => it.list = []
-  step it := pure (match it with
-        | ⟨[]⟩ => .deflate ⟨.done, rfl⟩
-        | ⟨x :: xs⟩ => .deflate ⟨.yield ⟨xs⟩ x, rfl⟩)
-
 /--
 Returns a finite iterator for the given list.
 The iterator yields the elements of the list in order and then terminates.
@@ -59,15 +47,25 @@ The iterator yields the elements of the list in order and then terminates.
 @[always_inline, inline]
 def List.iter {α : Type u} (l : List α) (m : Type u → Type w := by exact Id) [Pure m] :
     Iter (α := ListIterator α) m α :=
-  toIter m { list := l }
+  toIter { list := l } m α
+
+instance {α : Type u} [Pure m] [UnivLE.{u, w}] : Iterator (ListIterator α) m α where
+  value_small := inferInstance
+  plausible_step it
+    | .yield it' out => it.inner.list = out :: it'.inner.list
+    | .skip _ => False
+    | .done => it.inner.list = []
+  step it := letI l := it.inner; pure (match h : l with
+        | ⟨[]⟩ => .deflate ⟨.done, by simp_all [l]⟩
+        | ⟨x :: xs⟩ => .deflate ⟨.yield (toIter ⟨xs⟩ m α) x, (by simp_all [l])⟩)
 
 instance [Pure m] [UnivLE.{u, w}] : FinitenessRelation (ListIterator α) m where
-  rel := InvImage WellFoundedRelation.rel ListIterator.list
+  rel := InvImage WellFoundedRelation.rel (ListIterator.list ∘ Iter.inner)
   wf := InvImage.wf _ WellFoundedRelation.wf
   subrelation {it it'} h := by
     simp_wf
     obtain ⟨step, h, h'⟩ := h
-    cases step <;> simp_all [IterStep.successor, Iterator.plausible_step]
+    cases step <;> simp_all [IterStep.successor, Iter.plausible_step, Iterator.plausible_step]
 
 end ListIterator
 
@@ -81,13 +79,12 @@ structure UnfoldIterator (α : Type u) (f : α → α) where
   next : α
 
 instance [Pure m] [UnivLE.{u, w}] : Iterator (UnfoldIterator α f) m α where
-  state_small := inferInstance
   value_small := inferInstance
   plausible_step it
-    | .yield it' out => out = it.next ∧ it' = ⟨f it.next⟩
+    | .yield it' out => out = it.inner.next ∧ it' = toIter ⟨f it.inner.next⟩ m α
     | .skip _ => False
     | .done => False
-  step it := pure <| .deflate <| .yield ⟨f it.next⟩ it.next (by simp)
+  step it := pure <| .deflate <| .yield (toIter ⟨f it.inner.next⟩ m α) it.inner.next (by simp)
 
 /--
 Creates an infinite, productive iterator. First it yields `init`.
@@ -95,7 +92,7 @@ If the last step yielded `a`, the next will yield `f a`.
 -/
 @[inline]
 def Iter.unfold (m : Type u → Type w') [Pure m] {α : Type u} (init : α) (f : α → α) :=
-  toIter m <| UnfoldIterator.mk (f := f) init
+  toIter (UnfoldIterator.mk (f := f) init) m α
 
 instance [Pure m] [UnivLE.{u, w}] : ProductivenessRelation (UnfoldIterator α f) m where
   rel := emptyWf.rel
